bump to nightly-2023-01-18-12
mathlib commit https://github.com/leanprover-community/mathlib/commit/008205aa645b3f194c1da47025c5f110c8406eab

Mathbin/Data/Multiset/Sort.lean
@@ -26,47 +26,67 @@ section Sort
 
 variable (r : α → α → Prop) [DecidableRel r] [IsTrans α r] [IsAntisymm α r] [IsTotal α r]
 
+#print Multiset.sort /-
 /-- `sort s` constructs a sorted list from the multiset `s`.
   (Uses merge sort algorithm.) -/
 def sort (s : Multiset α) : List α :=
   Quot.liftOn s (mergeSort r) fun a b h =>
-    eq_of_perm_of_sorted ((perm_merge_sort _ _).trans <| h.trans (perm_merge_sort _ _).symm)
-      (sorted_merge_sort r _) (sorted_merge_sort r _)
+    eq_of_perm_of_sorted ((perm_mergeSort _ _).trans <| h.trans (perm_mergeSort _ _).symm)
+      (sorted_mergeSort r _) (sorted_mergeSort r _)
 #align multiset.sort Multiset.sort
+-/
 
+#print Multiset.coe_sort /-
 @[simp]
 theorem coe_sort (l : List α) : sort r l = mergeSort r l :=
   rfl
 #align multiset.coe_sort Multiset.coe_sort
+-/
 
+#print Multiset.sort_sorted /-
 @[simp]
 theorem sort_sorted (s : Multiset α) : Sorted r (sort r s) :=
-  Quot.inductionOn s fun l => sorted_merge_sort r _
+  Quot.inductionOn s fun l => sorted_mergeSort r _
 #align multiset.sort_sorted Multiset.sort_sorted
+-/
 
+#print Multiset.sort_eq /-
 @[simp]
 theorem sort_eq (s : Multiset α) : ↑(sort r s) = s :=
-  Quot.inductionOn s fun l => Quot.sound <| perm_merge_sort _ _
+  Quot.inductionOn s fun l => Quot.sound <| perm_mergeSort _ _
 #align multiset.sort_eq Multiset.sort_eq
+-/
 
+#print Multiset.mem_sort /-
 @[simp]
 theorem mem_sort {s : Multiset α} {a : α} : a ∈ sort r s ↔ a ∈ s := by rw [← mem_coe, sort_eq]
 #align multiset.mem_sort Multiset.mem_sort
+-/
 
+/- warning: multiset.length_sort -> Multiset.length_sort is a dubious translation:
+lean 3 declaration is
+  forall {α : Type.{u1}} (r : α -> α -> Prop) [_inst_1 : DecidableRel.{succ u1} α r] [_inst_2 : IsTrans.{u1} α r] [_inst_3 : IsAntisymm.{u1} α r] [_inst_4 : IsTotal.{u1} α r] {s : Multiset.{u1} α}, Eq.{1} Nat (List.length.{u1} α (Multiset.sort.{u1} α r (fun (a : α) (b : α) => _inst_1 a b) _inst_2 _inst_3 _inst_4 s)) (coeFn.{succ u1, succ u1} (AddMonoidHom.{u1, 0} (Multiset.{u1} α) Nat (AddMonoid.toAddZeroClass.{u1} (Multiset.{u1} α) (AddRightCancelMonoid.toAddMonoid.{u1} (Multiset.{u1} α) (AddCancelMonoid.toAddRightCancelMonoid.{u1} (Multiset.{u1} α) (AddCancelCommMonoid.toCancelAddMonoid.{u1} (Multiset.{u1} α) (OrderedCancelAddCommMonoid.toCancelAddCommMonoid.{u1} (Multiset.{u1} α) (Multiset.orderedCancelAddCommMonoid.{u1} α)))))) (AddMonoid.toAddZeroClass.{0} Nat Nat.addMonoid)) (fun (_x : AddMonoidHom.{u1, 0} (Multiset.{u1} α) Nat (AddMonoid.toAddZeroClass.{u1} (Multiset.{u1} α) (AddRightCancelMonoid.toAddMonoid.{u1} (Multiset.{u1} α) (AddCancelMonoid.toAddRightCancelMonoid.{u1} (Multiset.{u1} α) (AddCancelCommMonoid.toCancelAddMonoid.{u1} (Multiset.{u1} α) (OrderedCancelAddCommMonoid.toCancelAddCommMonoid.{u1} (Multiset.{u1} α) (Multiset.orderedCancelAddCommMonoid.{u1} α)))))) (AddMonoid.toAddZeroClass.{0} Nat Nat.addMonoid)) => (Multiset.{u1} α) -> Nat) (AddMonoidHom.hasCoeToFun.{u1, 0} (Multiset.{u1} α) Nat (AddMonoid.toAddZeroClass.{u1} (Multiset.{u1} α) (AddRightCancelMonoid.toAddMonoid.{u1} (Multiset.{u1} α) (AddCancelMonoid.toAddRightCancelMonoid.{u1} (Multiset.{u1} α) (AddCancelCommMonoid.toCancelAddMonoid.{u1} (Multiset.{u1} α) (OrderedCancelAddCommMonoid.toCancelAddCommMonoid.{u1} (Multiset.{u1} α) (Multiset.orderedCancelAddCommMonoid.{u1} α)))))) (AddMonoid.toAddZeroClass.{0} Nat Nat.addMonoid)) (Multiset.card.{u1} α) s)
+but is expected to have type
+  forall {α : Type.{u1}} (r : α -> α -> Prop) [_inst_1 : DecidableRel.{succ u1} α r] [_inst_2 : IsTrans.{u1} α r] [_inst_3 : IsAntisymm.{u1} α r] [_inst_4 : IsTotal.{u1} α r] {s : Multiset.{u1} α}, Eq.{1} Nat (List.length.{u1} α (Multiset.sort.{u1} α r (fun (a : α) (b : α) => _inst_1 a b) _inst_2 _inst_3 _inst_4 s)) (FunLike.coe.{succ u1, succ u1, 1} (AddMonoidHom.{u1, 0} (Multiset.{u1} α) Nat (AddMonoid.toAddZeroClass.{u1} (Multiset.{u1} α) (AddRightCancelMonoid.toAddMonoid.{u1} (Multiset.{u1} α) (AddCancelMonoid.toAddRightCancelMonoid.{u1} (Multiset.{u1} α) (AddCancelCommMonoid.toAddCancelMonoid.{u1} (Multiset.{u1} α) (OrderedCancelAddCommMonoid.toCancelAddCommMonoid.{u1} (Multiset.{u1} α) (Multiset.instOrderedCancelAddCommMonoidMultiset.{u1} α)))))) (AddMonoid.toAddZeroClass.{0} Nat Nat.addMonoid)) (Multiset.{u1} α) (fun (_x : Multiset.{u1} α) => (fun (x._@.Mathlib.Algebra.Hom.Group._hyg.398 : Multiset.{u1} α) => Nat) _x) (AddHomClass.toFunLike.{u1, u1, 0} (AddMonoidHom.{u1, 0} (Multiset.{u1} α) Nat (AddMonoid.toAddZeroClass.{u1} (Multiset.{u1} α) (AddRightCancelMonoid.toAddMonoid.{u1} (Multiset.{u1} α) (AddCancelMonoid.toAddRightCancelMonoid.{u1} (Multiset.{u1} α) (AddCancelCommMonoid.toAddCancelMonoid.{u1} (Multiset.{u1} α) (OrderedCancelAddCommMonoid.toCancelAddCommMonoid.{u1} (Multiset.{u1} α) (Multiset.instOrderedCancelAddCommMonoidMultiset.{u1} α)))))) (AddMonoid.toAddZeroClass.{0} Nat Nat.addMonoid)) (Multiset.{u1} α) Nat (AddZeroClass.toAdd.{u1} (Multiset.{u1} α) (AddMonoid.toAddZeroClass.{u1} (Multiset.{u1} α) (AddRightCancelMonoid.toAddMonoid.{u1} (Multiset.{u1} α) (AddCancelMonoid.toAddRightCancelMonoid.{u1} (Multiset.{u1} α) (AddCancelCommMonoid.toAddCancelMonoid.{u1} (Multiset.{u1} α) (OrderedCancelAddCommMonoid.toCancelAddCommMonoid.{u1} (Multiset.{u1} α) (Multiset.instOrderedCancelAddCommMonoidMultiset.{u1} α))))))) (AddZeroClass.toAdd.{0} Nat (AddMonoid.toAddZeroClass.{0} Nat Nat.addMonoid)) (AddMonoidHomClass.toAddHomClass.{u1, u1, 0} (AddMonoidHom.{u1, 0} (Multiset.{u1} α) Nat (AddMonoid.toAddZeroClass.{u1} (Multiset.{u1} α) (AddRightCancelMonoid.toAddMonoid.{u1} (Multiset.{u1} α) (AddCancelMonoid.toAddRightCancelMonoid.{u1} (Multiset.{u1} α) (AddCancelCommMonoid.toAddCancelMonoid.{u1} (Multiset.{u1} α) (OrderedCancelAddCommMonoid.toCancelAddCommMonoid.{u1} (Multiset.{u1} α) (Multiset.instOrderedCancelAddCommMonoidMultiset.{u1} α)))))) (AddMonoid.toAddZeroClass.{0} Nat Nat.addMonoid)) (Multiset.{u1} α) Nat (AddMonoid.toAddZeroClass.{u1} (Multiset.{u1} α) (AddRightCancelMonoid.toAddMonoid.{u1} (Multiset.{u1} α) (AddCancelMonoid.toAddRightCancelMonoid.{u1} (Multiset.{u1} α) (AddCancelCommMonoid.toAddCancelMonoid.{u1} (Multiset.{u1} α) (OrderedCancelAddCommMonoid.toCancelAddCommMonoid.{u1} (Multiset.{u1} α) (Multiset.instOrderedCancelAddCommMonoidMultiset.{u1} α)))))) (AddMonoid.toAddZeroClass.{0} Nat Nat.addMonoid) (AddMonoidHom.addMonoidHomClass.{u1, 0} (Multiset.{u1} α) Nat (AddMonoid.toAddZeroClass.{u1} (Multiset.{u1} α) (AddRightCancelMonoid.toAddMonoid.{u1} (Multiset.{u1} α) (AddCancelMonoid.toAddRightCancelMonoid.{u1} (Multiset.{u1} α) (AddCancelCommMonoid.toAddCancelMonoid.{u1} (Multiset.{u1} α) (OrderedCancelAddCommMonoid.toCancelAddCommMonoid.{u1} (Multiset.{u1} α) (Multiset.instOrderedCancelAddCommMonoidMultiset.{u1} α)))))) (AddMonoid.toAddZeroClass.{0} Nat Nat.addMonoid)))) (Multiset.card.{u1} α) s)
+Case conversion may be inaccurate. Consider using '#align multiset.length_sort Multiset.length_sortₓ'. -/
 @[simp]
 theorem length_sort {s : Multiset α} : (sort r s).length = s.card :=
-  Quot.inductionOn s <| length_merge_sort _
+  Quot.inductionOn s <| length_mergeSort _
 #align multiset.length_sort Multiset.length_sort
 
+#print Multiset.sort_zero /-
 @[simp]
 theorem sort_zero : sort r 0 = [] :=
-  List.merge_sort_nil r
+  List.mergeSort_nil r
 #align multiset.sort_zero Multiset.sort_zero
+-/
 
+#print Multiset.sort_singleton /-
 @[simp]
 theorem sort_singleton (a : α) : sort r {a} = [a] :=
-  List.merge_sort_singleton r a
+  List.mergeSort_singleton r a
 #align multiset.sort_singleton Multiset.sort_singleton
+-/
 
 end Sort
 
