Mathbin/Data/List/Sort.lean
@@ -35,43 +35,60 @@ section Sorted
 
 variable {α : Type uu} {r : α → α → Prop} {a : α} {l : List α}
 
+#print List.Sorted /-
 /-- `sorted r l` is the same as `pairwise r l`, preferred in the case that `r`
   is a `<` or `≤`-like relation (transitive and antisymmetric or asymmetric) -/
 def Sorted :=
   @Pairwise
 #align list.sorted List.Sorted
+-/
 
+#print List.decidableSorted /-
 instance decidableSorted [DecidableRel r] (l : List α) : Decidable (Sorted r l) :=
   List.instDecidablePairwise _
 #align list.decidable_sorted List.decidableSorted
+-/
 
+#print List.sorted_nil /-
 @[simp]
 theorem sorted_nil : Sorted r [] :=
   pairwise.nil
 #align list.sorted_nil List.sorted_nil
+-/
 
+#print List.Sorted.of_cons /-
 theorem Sorted.of_cons : Sorted r (a :: l) → Sorted r l :=
   pairwise.of_cons
 #align list.sorted.of_cons List.Sorted.of_cons
+-/
 
+#print List.Sorted.tail /-
 theorem Sorted.tail {r : α → α → Prop} {l : List α} (h : Sorted r l) : Sorted r l.tail :=
   h.tail
 #align list.sorted.tail List.Sorted.tail
+-/
 
+#print List.rel_of_sorted_cons /-
 theorem rel_of_sorted_cons {a : α} {l : List α} : Sorted r (a :: l) → ∀ b ∈ l, r a b :=
   rel_of_pairwise_cons
 #align list.rel_of_sorted_cons List.rel_of_sorted_cons
+-/
 
+#print List.sorted_cons /-
 @[simp]
 theorem sorted_cons {a : α} {l : List α} : Sorted r (a :: l) ↔ (∀ b ∈ l, r a b) ∧ Sorted r l :=
   pairwise_cons
 #align list.sorted_cons List.sorted_cons
+-/
 
+#print List.Sorted.nodup /-
 protected theorem Sorted.nodup {r : α → α → Prop} [IsIrrefl α r] {l : List α} (h : Sorted r l) :
     Nodup l :=
   h.Nodup
 #align list.sorted.nodup List.Sorted.nodup
+-/
 
+#print List.eq_of_perm_of_sorted /-
 theorem eq_of_perm_of_sorted [IsAntisymm α r] {l₁ l₂ : List α} (p : l₁ ~ l₂) (s₁ : Sorted r l₁)
     (s₂ : Sorted r l₂) : l₁ = l₂ :=
   by
@@ -91,33 +108,43 @@ theorem eq_of_perm_of_sorted [IsAntisymm α r] {l₁ l₂ : List α} (p : l₁ ~
         constructor <;>
       simp [iff_true_intro this, or_comm']
 #align list.eq_of_perm_of_sorted List.eq_of_perm_of_sorted
+-/
 
+#print List.sublist_of_subperm_of_sorted /-
 theorem sublist_of_subperm_of_sorted [IsAntisymm α r] {l₁ l₂ : List α} (p : l₁ <+~ l₂)
     (s₁ : l₁.Sorted r) (s₂ : l₂.Sorted r) : l₁ <+ l₂ :=
   by
   let ⟨_, h, h'⟩ := p
   rwa [← eq_of_perm_of_sorted h (s₂.sublist h') s₁]
 #align list.sublist_of_subperm_of_sorted List.sublist_of_subperm_of_sorted
+-/
 
+#print List.sorted_singleton /-
 @[simp]
 theorem sorted_singleton (a : α) : Sorted r [a] :=
   pairwise_singleton _ _
 #align list.sorted_singleton List.sorted_singleton
+-/
 
-theorem Sorted.rel_nth_le_of_lt {l : List α} (h : l.Sorted r) {a b : ℕ} (ha : a < l.length)
+#print List.Sorted.rel_nthLe_of_lt /-
+theorem Sorted.rel_nthLe_of_lt {l : List α} (h : l.Sorted r) {a b : ℕ} (ha : a < l.length)
     (hb : b < l.length) (hab : a < b) : r (l.nthLe a ha) (l.nthLe b hb) :=
   List.pairwise_iff_nthLe.1 h a b hb hab
-#align list.sorted.rel_nth_le_of_lt List.Sorted.rel_nth_le_of_lt
+#align list.sorted.rel_nth_le_of_lt List.Sorted.rel_nthLe_of_lt
+-/
 
-theorem Sorted.rel_nth_le_of_le [IsRefl α r] {l : List α} (h : l.Sorted r) {a b : ℕ}
+#print List.Sorted.rel_nthLe_of_le /-
+theorem Sorted.rel_nthLe_of_le [IsRefl α r] {l : List α} (h : l.Sorted r) {a b : ℕ}
     (ha : a < l.length) (hb : b < l.length) (hab : a ≤ b) : r (l.nthLe a ha) (l.nthLe b hb) :=
   by
   cases' eq_or_lt_of_le hab with H H
   · subst H
     exact refl _
   · exact h.rel_nth_le_of_lt _ _ H
-#align list.sorted.rel_nth_le_of_le List.Sorted.rel_nth_le_of_le
+#align list.sorted.rel_nth_le_of_le List.Sorted.rel_nthLe_of_le
+-/
 
+#print List.Sorted.rel_of_mem_take_of_mem_drop /-
 theorem Sorted.rel_of_mem_take_of_mem_drop {l : List α} (h : List.Sorted r l) {k : ℕ} {x y : α}
     (hx : x ∈ List.take k l) (hy : y ∈ List.drop k l) : r x y :=
   by
@@ -127,6 +154,7 @@ theorem Sorted.rel_of_mem_take_of_mem_drop {l : List α} (h : List.Sorted r l) {
   rw [length_take] at hix
   exact h.rel_nth_le_of_lt _ _ (ix.lt_add_right _ _ (lt_min_iff.mp hix).left)
 #align list.sorted.rel_of_mem_take_of_mem_drop List.Sorted.rel_of_mem_take_of_mem_drop
+-/
 
 end Sorted
 
@@ -134,17 +162,29 @@ section Monotone
 
 variable {n : ℕ} {α : Type uu} [Preorder α] {f : Fin n → α}
 
+/- warning: list.monotone_iff_of_fn_sorted -> List.monotone_iff_ofFn_sorted is a dubious translation:
+lean 3 declaration is
+  forall {n : Nat} {α : Type.{u1}} [_inst_1 : Preorder.{u1} α] {f : (Fin n) -> α}, Iff (Monotone.{0, u1} (Fin n) α (PartialOrder.toPreorder.{0} (Fin n) (Fin.partialOrder n)) _inst_1 f) (List.Sorted.{u1} α (LE.le.{u1} α (Preorder.toLE.{u1} α _inst_1)) (List.ofFn.{u1} α n f))
+but is expected to have type
+  forall {n : Nat} {α : Type.{u1}} [_inst_1 : Preorder.{u1} α] {f : (Fin n) -> α}, Iff (Monotone.{0, u1} (Fin n) α (PartialOrder.toPreorder.{0} (Fin n) (Fin.instPartialOrderFin n)) _inst_1 f) (List.Sorted.{u1} α (fun (x._@.Mathlib.Data.List.Sort._hyg.1089 : α) (x._@.Mathlib.Data.List.Sort._hyg.1091 : α) => LE.le.{u1} α (Preorder.toLE.{u1} α _inst_1) x._@.Mathlib.Data.List.Sort._hyg.1089 x._@.Mathlib.Data.List.Sort._hyg.1091) (List.ofFn.{u1} α n f))
+Case conversion may be inaccurate. Consider using '#align list.monotone_iff_of_fn_sorted List.monotone_iff_ofFn_sortedₓ'. -/
 /-- A tuple is monotone if and only if the list obtained from it is sorted. -/
-theorem monotone_iff_of_fn_sorted : Monotone f ↔ (ofFn f).Sorted (· ≤ ·) :=
+theorem monotone_iff_ofFn_sorted : Monotone f ↔ (ofFn f).Sorted (· ≤ ·) :=
   by
   simp_rw [sorted, pairwise_iff_nth_le, length_of_fn, nth_le_of_fn', monotone_iff_forall_lt]
   exact ⟨fun h i j hj hij => h <| fin.mk_lt_mk.mpr hij, fun h ⟨i, _⟩ ⟨j, hj⟩ hij => h i j hj hij⟩
-#align list.monotone_iff_of_fn_sorted List.monotone_iff_of_fn_sorted
+#align list.monotone_iff_of_fn_sorted List.monotone_iff_ofFn_sorted
 
+/- warning: list.monotone.of_fn_sorted -> List.Monotone.ofFn_sorted is a dubious translation:
+lean 3 declaration is
+  forall {n : Nat} {α : Type.{u1}} [_inst_1 : Preorder.{u1} α] {f : (Fin n) -> α}, (Monotone.{0, u1} (Fin n) α (PartialOrder.toPreorder.{0} (Fin n) (Fin.partialOrder n)) _inst_1 f) -> (List.Sorted.{u1} α (LE.le.{u1} α (Preorder.toLE.{u1} α _inst_1)) (List.ofFn.{u1} α n f))
+but is expected to have type
+  forall {n : Nat} {α : Type.{u1}} [_inst_1 : Preorder.{u1} α] {f : (Fin n) -> α}, (Monotone.{0, u1} (Fin n) α (PartialOrder.toPreorder.{0} (Fin n) (Fin.instPartialOrderFin n)) _inst_1 f) -> (List.Sorted.{u1} α (fun (x._@.Mathlib.Data.List.Sort._hyg.1229 : α) (x._@.Mathlib.Data.List.Sort._hyg.1231 : α) => LE.le.{u1} α (Preorder.toLE.{u1} α _inst_1) x._@.Mathlib.Data.List.Sort._hyg.1229 x._@.Mathlib.Data.List.Sort._hyg.1231) (List.ofFn.{u1} α n f))
+Case conversion may be inaccurate. Consider using '#align list.monotone.of_fn_sorted List.Monotone.ofFn_sortedₓ'. -/
 /-- The list obtained from a monotone tuple is sorted. -/
-theorem Monotone.of_fn_sorted (h : Monotone f) : (ofFn f).Sorted (· ≤ ·) :=
-  monotone_iff_of_fn_sorted.1 h
-#align list.monotone.of_fn_sorted List.Monotone.of_fn_sorted
+theorem Monotone.ofFn_sorted (h : Monotone f) : (ofFn f).Sorted (· ≤ ·) :=
+  monotone_iff_ofFn_sorted.1 h
+#align list.monotone.of_fn_sorted List.Monotone.ofFn_sorted
 
 end Monotone
 
@@ -160,6 +200,7 @@ local infixl:50 " ≼ " => r
 
 section InsertionSort
 
+#print List.orderedInsert /-
 /-- `ordered_insert a l` inserts `a` into `l` at such that
   `ordered_insert a l` is sorted if `l` is. -/
 @[simp]
@@ -167,85 +208,105 @@ def orderedInsert (a : α) : List α → List α
   | [] => [a]
   | b :: l => if a ≼ b then a :: b :: l else b :: ordered_insert l
 #align list.ordered_insert List.orderedInsert
+-/
 
+#print List.insertionSort /-
 /-- `insertion_sort l` returns `l` sorted using the insertion sort algorithm. -/
 @[simp]
 def insertionSort : List α → List α
   | [] => []
   | b :: l => orderedInsert r b (insertion_sort l)
 #align list.insertion_sort List.insertionSort
+-/
 
+#print List.orderedInsert_nil /-
 @[simp]
-theorem ordered_insert_nil (a : α) : [].orderedInsert r a = [a] :=
+theorem orderedInsert_nil (a : α) : [].orderedInsert r a = [a] :=
   rfl
-#align list.ordered_insert_nil List.ordered_insert_nil
+#align list.ordered_insert_nil List.orderedInsert_nil
+-/
 
-theorem ordered_insert_length : ∀ (L : List α) (a : α), (L.orderedInsert r a).length = L.length + 1
+#print List.orderedInsert_length /-
+theorem orderedInsert_length : ∀ (L : List α) (a : α), (L.orderedInsert r a).length = L.length + 1
   | [], a => rfl
   | hd :: tl, a => by
     dsimp [ordered_insert]
     split_ifs <;> simp [ordered_insert_length]
-#align list.ordered_insert_length List.ordered_insert_length
+#align list.ordered_insert_length List.orderedInsert_length
+-/
 
+#print List.orderedInsert_eq_take_drop /-
 /-- An alternative definition of `ordered_insert` using `take_while` and `drop_while`. -/
-theorem ordered_insert_eq_take_drop (a : α) :
+theorem orderedInsert_eq_take_drop (a : α) :
     ∀ l : List α,
       l.orderedInsert r a = (l.takeWhile fun b => ¬a ≼ b) ++ a :: l.dropWhile fun b => ¬a ≼ b
   | [] => rfl
   | b :: l => by
     dsimp only [ordered_insert]
     split_ifs <;> simp [take_while, drop_while, *]
-#align list.ordered_insert_eq_take_drop List.ordered_insert_eq_take_drop
+#align list.ordered_insert_eq_take_drop List.orderedInsert_eq_take_drop
+-/
 
-theorem insertion_sort_cons_eq_take_drop (a : α) (l : List α) :
+#print List.insertionSort_cons_eq_take_drop /-
+theorem insertionSort_cons_eq_take_drop (a : α) (l : List α) :
     insertionSort r (a :: l) =
       ((insertionSort r l).takeWhile fun b => ¬a ≼ b) ++
         a :: (insertionSort r l).dropWhile fun b => ¬a ≼ b :=
-  ordered_insert_eq_take_drop r a _
-#align list.insertion_sort_cons_eq_take_drop List.insertion_sort_cons_eq_take_drop
+  orderedInsert_eq_take_drop r a _
+#align list.insertion_sort_cons_eq_take_drop List.insertionSort_cons_eq_take_drop
+-/
 
 section Correctness
 
 open Perm
 
-theorem perm_ordered_insert (a) : ∀ l : List α, orderedInsert r a l ~ a :: l
+#print List.perm_orderedInsert /-
+theorem perm_orderedInsert (a) : ∀ l : List α, orderedInsert r a l ~ a :: l
   | [] => Perm.refl _
   | b :: l => by
     by_cases a ≼ b <;> [simp [ordered_insert, h],
       simpa [ordered_insert, h] using ((perm_ordered_insert l).cons _).trans (perm.swap _ _ _)]
-#align list.perm_ordered_insert List.perm_ordered_insert
+#align list.perm_ordered_insert List.perm_orderedInsert
+-/
 
-theorem ordered_insert_count [DecidableEq α] (L : List α) (a b : α) :
+#print List.orderedInsert_count /-
+theorem orderedInsert_count [DecidableEq α] (L : List α) (a b : α) :
     count a (L.orderedInsert r b) = count a L + if a = b then 1 else 0 :=
   by
   rw [(L.perm_ordered_insert r b).count_eq, count_cons]
   split_ifs <;> simp only [Nat.succ_eq_add_one, add_zero]
-#align list.ordered_insert_count List.ordered_insert_count
+#align list.ordered_insert_count List.orderedInsert_count
+-/
 
-theorem perm_insertion_sort : ∀ l : List α, insertionSort r l ~ l
+#print List.perm_insertionSort /-
+theorem perm_insertionSort : ∀ l : List α, insertionSort r l ~ l
   | [] => Perm.nil
   | b :: l => by
     simpa [insertion_sort] using (perm_ordered_insert _ _ _).trans ((perm_insertion_sort l).cons b)
-#align list.perm_insertion_sort List.perm_insertion_sort
+#align list.perm_insertion_sort List.perm_insertionSort
+-/
 
 variable {r}
 
+#print List.Sorted.insertionSort_eq /-
 /-- If `l` is already `list.sorted` with respect to `r`, then `insertion_sort` does not change
 it. -/
-theorem Sorted.insertion_sort_eq : ∀ {l : List α} (h : Sorted r l), insertionSort r l = l
+theorem Sorted.insertionSort_eq : ∀ {l : List α} (h : Sorted r l), insertionSort r l = l
   | [], _ => rfl
   | [a], _ => rfl
   | a :: b :: l, h =>
     by
     rw [insertion_sort, sorted.insertion_sort_eq, ordered_insert, if_pos]
     exacts[rel_of_sorted_cons h _ (Or.inl rfl), h.tail]
-#align list.sorted.insertion_sort_eq List.Sorted.insertion_sort_eq
+#align list.sorted.insertion_sort_eq List.Sorted.insertionSort_eq
+-/
 
 section TotalAndTransitive
 
 variable [IsTotal α r] [IsTrans α r]
 
-theorem Sorted.ordered_insert (a : α) : ∀ l, Sorted r l → Sorted r (orderedInsert r a l)
+#print List.Sorted.orderedInsert /-
+theorem Sorted.orderedInsert (a : α) : ∀ l, Sorted r l → Sorted r (orderedInsert r a l)
   | [], h => sorted_singleton a
   | b :: l, h => by
     by_cases h' : a ≼ b
@@ -257,15 +318,18 @@ theorem Sorted.ordered_insert (a : α) : ∀ l, Sorted r l → Sorted r (ordered
       · subst b'
         exact (total_of r _ _).resolve_left h'
       · exact rel_of_sorted_cons h _ bm
-#align list.sorted.ordered_insert List.Sorted.ordered_insert
+#align list.sorted.ordered_insert List.Sorted.orderedInsert
+-/
 
 variable (r)
 
+#print List.sorted_insertionSort /-
 /-- The list `list.insertion_sort r l` is `list.sorted` with respect to `r`. -/
-theorem sorted_insertion_sort : ∀ l, Sorted r (insertionSort r l)
+theorem sorted_insertionSort : ∀ l, Sorted r (insertionSort r l)
   | [] => sorted_nil
   | a :: l => (sorted_insertion_sort l).orderedInsert a _
-#align list.sorted_insertion_sort List.sorted_insertion_sort
+#align list.sorted_insertion_sort List.sorted_insertionSort
+-/
 
 end TotalAndTransitive
 
@@ -278,6 +342,7 @@ end InsertionSort
 
 section MergeSort
 
+#print List.split /-
 -- TODO(Jeremy): observation: if instead we write (a :: (split l).1, b :: (split l).2), the
 -- equation compiler can't prove the third equation
 /-- Split `l` into two lists of approximately equal length.
@@ -290,11 +355,15 @@ def split : List α → List α × List α
     let (l₁, l₂) := split l
     (a :: l₂, l₁)
 #align list.split List.split
+-/
 
+#print List.split_cons_of_eq /-
 theorem split_cons_of_eq (a : α) {l l₁ l₂ : List α} (h : split l = (l₁, l₂)) :
     split (a :: l) = (a :: l₂, l₁) := by rw [split, h] <;> rfl
 #align list.split_cons_of_eq List.split_cons_of_eq
+-/
 
+#print List.length_split_le /-
 theorem length_split_le :
     ∀ {l l₁ l₂ : List α}, split l = (l₁, l₂) → length l₁ ≤ length l ∧ length l₂ ≤ length l
   | [], _, _, rfl => ⟨Nat.le_refl 0, Nat.le_refl 0⟩
@@ -304,7 +373,9 @@ theorem length_split_le :
     cases' length_split_le e with h₁ h₂
     exact ⟨Nat.succ_le_succ h₂, Nat.le_succ_of_le h₁⟩
 #align list.length_split_le List.length_split_le
+-/
 
+#print List.length_split_lt /-
 theorem length_split_lt {a b} {l l₁ l₂ : List α} (h : split (a :: b :: l) = (l₁, l₂)) :
     length l₁ < length (a :: b :: l) ∧ length l₂ < length (a :: b :: l) :=
   by
@@ -313,7 +384,9 @@ theorem length_split_lt {a b} {l l₁ l₂ : List α} (h : split (a :: b :: l) =
   cases' length_split_le e with h₁ h₂
   exact ⟨Nat.succ_le_succ (Nat.succ_le_succ h₁), Nat.succ_le_succ (Nat.succ_le_succ h₂)⟩
 #align list.length_split_lt List.length_split_lt
+-/
 
+#print List.perm_split /-
 theorem perm_split : ∀ {l l₁ l₂ : List α}, split l = (l₁, l₂) → l ~ l₁ ++ l₂
   | [], _, _, rfl => Perm.refl _
   | a :: l, l₁', l₂', h => by
@@ -321,7 +394,9 @@ theorem perm_split : ∀ {l l₁ l₂ : List α}, split l = (l₁, l₂) → l ~
     injection (split_cons_of_eq _ e).symm.trans h; substs l₁' l₂'
     exact ((perm_split e).trans perm_append_comm).cons a
 #align list.perm_split List.perm_split
+-/
 
+#print List.merge /-
 /-- Merge two sorted lists into one in linear time.
 
      merge [1, 2, 4, 5] [0, 1, 3, 4] = [0, 1, 1, 2, 3, 4, 4, 5] -/
@@ -330,9 +405,11 @@ def merge : List α → List α → List α
   | l, [] => l
   | a :: l, b :: l' => if a ≼ b then a :: merge l (b :: l') else b :: merge (a :: l) l'
 #align list.merge List.merge
+-/
 
 include r
 
+#print List.mergeSort /-
 /-- Implementation of a merge sort algorithm to sort a list. -/
 def mergeSort : List α → List α
   | [] => []
@@ -343,8 +420,10 @@ def mergeSort : List α → List α
     exact merge r (merge_sort l₁) (merge_sort l₂)termination_by'
   ⟨_, InvImage.wf length Nat.lt_wfRel⟩
 #align list.merge_sort List.mergeSort
+-/
 
-theorem merge_sort_cons_cons {a b} {l l₁ l₂ : List α} (h : split (a :: b :: l) = (l₁, l₂)) :
+#print List.mergeSort_cons_cons /-
+theorem mergeSort_cons_cons {a b} {l l₁ l₂ : List α} (h : split (a :: b :: l) = (l₁, l₂)) :
     mergeSort r (a :: b :: l) = merge r (mergeSort r l₁) (mergeSort r l₂) :=
   by
   suffices
@@ -358,10 +437,12 @@ theorem merge_sort_cons_cons {a b} {l l₁ l₂ : List α} (h : split (a :: b ::
   intros
   cases h1
   rfl
-#align list.merge_sort_cons_cons List.merge_sort_cons_cons
+#align list.merge_sort_cons_cons List.mergeSort_cons_cons
+-/
 
 section Correctness
 
+#print List.perm_merge /-
 theorem perm_merge : ∀ l l' : List α, merge r l l' ~ l ++ l'
   | [], [] => by simp [merge]
   | [], b :: l' => by simp [merge]
@@ -372,8 +453,10 @@ theorem perm_merge : ∀ l l' : List α, merge r l l' ~ l ++ l'
     · suffices b :: merge r (a :: l) l' ~ a :: (l ++ b :: l') by simpa [merge, h]
       exact ((perm_merge _ _).cons _).trans ((swap _ _ _).trans (perm_middle.symm.cons _))
 #align list.perm_merge List.perm_merge
+-/
 
-theorem perm_merge_sort : ∀ l : List α, mergeSort r l ~ l
+#print List.perm_mergeSort /-
+theorem perm_mergeSort : ∀ l : List α, mergeSort r l ~ l
   | [] => by simp [merge_sort]
   | [a] => by simp [merge_sort]
   | a :: b :: l => by
@@ -384,17 +467,21 @@ theorem perm_merge_sort : ∀ l : List α, mergeSort r l ~ l
     exact
       ((perm_merge_sort l₁).append (perm_merge_sort l₂)).trans (perm_split e).symm termination_by'
   ⟨_, InvImage.wf length Nat.lt_wfRel⟩
-#align list.perm_merge_sort List.perm_merge_sort
+#align list.perm_merge_sort List.perm_mergeSort
+-/
 
+#print List.length_mergeSort /-
 @[simp]
-theorem length_merge_sort (l : List α) : (mergeSort r l).length = l.length :=
-  (perm_merge_sort r _).length_eq
-#align list.length_merge_sort List.length_merge_sort
+theorem length_mergeSort (l : List α) : (mergeSort r l).length = l.length :=
+  (perm_mergeSort r _).length_eq
+#align list.length_merge_sort List.length_mergeSort
+-/
 
 section TotalAndTransitive
 
 variable {r} [IsTotal α r] [IsTrans α r]
 
+#print List.Sorted.merge /-
 theorem Sorted.merge : ∀ {l l' : List α}, Sorted r l → Sorted r l' → Sorted r (merge r l l')
   | [], [], h₁, h₂ => by simp [merge]
   | [], b :: l', h₁, h₂ => by simpa [merge] using h₂
@@ -422,10 +509,12 @@ theorem Sorted.merge : ∀ {l l' : List α}, Sorted r l → Sorted r l' → Sort
       · exact trans ba (rel_of_sorted_cons h₁ _ bl)
       · exact rel_of_sorted_cons h₂ _ bl'
 #align list.sorted.merge List.Sorted.merge
+-/
 
 variable (r)
 
-theorem sorted_merge_sort : ∀ l : List α, Sorted r (mergeSort r l)
+#print List.sorted_mergeSort /-
+theorem sorted_mergeSort : ∀ l : List α, Sorted r (mergeSort r l)
   | [] => by simp [merge_sort]
   | [a] => by simp [merge_sort]
   | a :: b :: l => by
@@ -434,29 +523,38 @@ theorem sorted_merge_sort : ∀ l : List α, Sorted r (mergeSort r l)
     rw [merge_sort_cons_cons r e]
     exact (sorted_merge_sort l₁).merge (sorted_merge_sort l₂)termination_by'
   ⟨_, InvImage.wf length Nat.lt_wfRel⟩
-#align list.sorted_merge_sort List.sorted_merge_sort
+#align list.sorted_merge_sort List.sorted_mergeSort
+-/
 
-theorem merge_sort_eq_self [IsAntisymm α r] {l : List α} : Sorted r l → mergeSort r l = l :=
-  eq_of_perm_of_sorted (perm_merge_sort _ _) (sorted_merge_sort _ _)
-#align list.merge_sort_eq_self List.merge_sort_eq_self
+#print List.mergeSort_eq_self /-
+theorem mergeSort_eq_self [IsAntisymm α r] {l : List α} : Sorted r l → mergeSort r l = l :=
+  eq_of_perm_of_sorted (perm_mergeSort _ _) (sorted_mergeSort _ _)
+#align list.merge_sort_eq_self List.mergeSort_eq_self
+-/
 
-theorem merge_sort_eq_insertion_sort [IsAntisymm α r] (l : List α) :
+#print List.mergeSort_eq_insertionSort /-
+theorem mergeSort_eq_insertionSort [IsAntisymm α r] (l : List α) :
     mergeSort r l = insertionSort r l :=
-  eq_of_perm_of_sorted ((perm_merge_sort r l).trans (perm_insertion_sort r l).symm)
-    (sorted_merge_sort r l) (sorted_insertion_sort r l)
-#align list.merge_sort_eq_insertion_sort List.merge_sort_eq_insertion_sort
+  eq_of_perm_of_sorted ((perm_mergeSort r l).trans (perm_insertionSort r l).symm)
+    (sorted_mergeSort r l) (sorted_insertionSort r l)
+#align list.merge_sort_eq_insertion_sort List.mergeSort_eq_insertionSort
+-/
 
 end TotalAndTransitive
 
 end Correctness
 
+#print List.mergeSort_nil /-
 @[simp]
-theorem merge_sort_nil : [].mergeSort r = [] := by rw [List.mergeSort]
-#align list.merge_sort_nil List.merge_sort_nil
+theorem mergeSort_nil : [].mergeSort r = [] := by rw [List.mergeSort]
+#align list.merge_sort_nil List.mergeSort_nil
+-/
 
+#print List.mergeSort_singleton /-
 @[simp]
-theorem merge_sort_singleton (a : α) : [a].mergeSort r = [a] := by rw [List.mergeSort]
-#align list.merge_sort_singleton List.merge_sort_singleton
+theorem mergeSort_singleton (a : α) : [a].mergeSort r = [a] := by rw [List.mergeSort]
+#align list.merge_sort_singleton List.mergeSort_singleton
+-/
 
 end MergeSort
 
